Generalize diamond lemmas to splitpaths type class

uniana/disj/DiamondIncl.v
@@ -1,186 +1,9 @@
-Require Export DiamondPaths.
+Require Export SpathIncl.
 Require Import Lia.
-
-Definition sub_tag i j := |i| = |j| /\ hd 0 i <= hd 0 j /\ tl i = tl j.
-
-Lemma Tagle_len: forall [i j : Tag], i ⊴ j -> | i | = | j |.
-Proof.
-  intros. destruct H.
-  - eapply Taglt_len;eauto.
-  - subst. reflexivity.
-Qed.
-
-Lemma jj_subtag `(DiamondPaths)
-      (Hjle : j1 ⊴ j2)
-  : sub_tag j1 j2.
-Proof.
-  split;[|split].
-  - eapply Tagle_len;eauto.
-  - destruct Hjle;[|subst;eauto].
-    destruct H0;cbn;try lia.
-    exfalso.
-    eapply tl_eq in H. cbn in H. subst. eapply Taglt_irrefl;eauto.
-  - eapply tl_eq;eauto.
-Qed.
-
-Hint Resolve jj_subtag : diamond.
-
-Lemma loop_tag_dom_eq `(C : redCFG) (h p : Lab) (i j : Tag) t
-      (Hloop : loop_contains h p)
-      (Hpath : TPath (root,start_tag) (p,i) t)
-      (Htagle : j = take_r (depth h) i)
-      (Hdep : |j| = depth h)
-  : (h,j) ∈ t.
-Proof.
-  subst j.
-  clear Hdep.
-  revert h p i Hloop Hpath.
-  induction t;intros.
-  + inv Hpath.
-  + unfold TPath in Hpath. path_simpl' Hpath. destruct t.
-    {
-      eapply path_single in Hpath. destruct Hpath.
-      inversion H. subst p i. eapply root_no_loop in Hloop. contradiction.
-    }
-    inv_path Hpath. destruct c as [q j].
-    specialize (IHt) with (p:=q) (i:=j).
-    eapply tcfg_edge_destruct' in H0.
-    destruct H0 as [H0|[H0|[H0|H0]]].
-    all: destruct H0 as [Htag Hedge].
-    * subst. right.
-      eapply IHt. all:cycle 1.
-      -- eapply H.
-      -- eapply basic_edge_eq_loop in Hedge. rewrite Hedge. assumption.
-    * eapply deq_loop_entry_or in Hedge;eauto.
-      destruct Hedge.
-      -- subst. right.
-         rewrite take_r_cons_drop.
-         2: {
-           eapply loop_contains_deq_loop in H0.
-           eapply tag_depth' in H. rewrite H.
-           eapply deq_loop_depth;eauto.
-         }
-         eapply IHt;eauto.
-      -- subst p. left. rewrite take_r_geq;eauto.
-         eapply tag_depth' in Hpath. lia.
-    * destruct j.
-      {
-        eapply tag_depth' in H. cbn in H. eapply loop_contains_depth_lt in Hloop.
-        eapply back_edge_eq_loop in Hedge. rewrite Hedge in H. lia.
-      }
-      cbn in Htag. subst i.
-      decide (h = p).
-      -- subst p. left. rewrite take_r_geq;eauto.
-         eapply tag_depth' in Hpath. lia.
-      -- right. rewrite take_r_cons_replace with (b:=n).
-         2: {
-           copy Hedge Hedge'.
-           eapply back_edge_eq_loop in Hedge.
-           copy Hloop Hloop'.
-           eapply loop_contains_deq_loop in Hloop.
-           eapply eq_loop1 in Hloop;eauto. 2: symmetry;eauto.
-           eapply tag_depth' in H.
-           enough (depth h < S (| j |)).
-           { cbn in H. rewrite H in H0. lia. }
-           eapply deq_loop_depth in Hloop.
-           eapply le_lt_or_eq in Hloop.
-           destruct Hloop.
-           ++ cbn in H. lia.
-           ++ exfalso. rewrite Hedge in H0.
-              eapply loop_contains_deq_loop in Hloop' as Hdeq.
-              eapply deq_loop_depth_eq in H0;eauto.
-              eapply n0. eapply head_unique;eauto.
-              ** eapply loop_contains_ledge;eauto.
-              ** split;eauto.
-         }
-         eapply IHt;eauto.
-         eapply back_edge_eq_loop in Hedge. rewrite Hedge. eauto.
-    * subst.
-      destruct j.
-      {
-        eapply tag_depth' in H. cbn in H. eapply loop_contains_depth_lt in Hloop.
-        destruct Hedge. eapply deq_loop_exited in H0. eapply deq_loop_depth in H0. lia.
-      }
-      right. rewrite <-take_r_cons_drop with (a:=n).
-      all: cbn.
-      2: {
-        eapply tag_depth' in H. cbn in H.
-        enough (depth h < S (|j|)) by lia.
-        rewrite H.
-        eapply depth_exit in Hedge.
-        eapply loop_contains_deq_loop in Hloop. eapply deq_loop_depth in Hloop.
-        lia.
-      }
-      eapply IHt;eauto.
-      destruct Hedge. eapply deq_loop_exited in H0. eapply H0. eauto.
-Qed.
-
-Lemma loop_tag_dom_same `(C : redCFG) (h : Lab) (i j : Tag) t
-      (Hloop : loop_head h)
-      (Hpath : TPath (root,start_tag) (h,i) t)
-      (Htagle : sub_tag j i)
-  : (h,j) ∈ t.
-Proof.
-  destruct Htagle as [Hlen [Hhd Htl]].
-  destruct i,j;cbn in *;[|congruence|congruence|].
-  { eapply tag_depth' in Hpath. cbn in Hpath. eapply depth_loop_head in Hloop. lia. }
-  subst j. clear Hlen.
-  revert t Hpath.
-  induction Hhd;intros.
-  - eapply path_contains_front;eauto.
-  - destruct t;[inv Hpath|].
-    unfold TPath in Hpath. path_simpl' Hpath.
-    inversion Hpath. subst.
-    destruct b as [q j].
-    eapply tcfg_edge_destruct' in H3.
-      destruct H3 as [H3|[H3|[H3|H3]]].
-      all: destruct H3 as [Htag Hedge].
-      * eapply basic_edge_no_loop2 in Hedge. contradiction.
-      * inv Htag.
-      * destruct j;cbn in Htag;[congruence|].
-        inv Htag.
-        right.
-        eapply loop_tag_dom_eq in H0 as Hel2;cycle 1.
-        -- eapply loop_contains_ledge;eassumption.
-        -- rewrite take_r_geq;eauto. eapply tag_depth' in H0. rewrite H0.
-           eapply back_edge_eq_loop in Hedge. rewrite Hedge. eauto.
-        -- eapply back_edge_eq_loop in Hedge. rewrite <-Hedge. eapply tag_depth' in H0. eauto.
-        -- eapply path_to_elem in Hel2;eauto. destructH.
-           eapply prefix_incl;[eauto|].
-           eapply IHHhd;eassumption.
-      * destruct j;cbn in Htag;[congruence|]. subst j. destruct Hedge.
-        eapply no_exit_head in H. contradiction.
-Qed.
-
-(* could be generalized with sub_tag _ _  -> sub_tag _ _ \/ Prefix _ _ *)
-Lemma loop_tag_dom `(C : redCFG) (h p : Lab) (i j : Tag) t
-      (Hloop : loop_contains h p)
-      (Hpath : TPath (root,start_tag) (p,i) t)
-      (Hstag : sub_tag j (take_r (depth h) i))
-      (Hdep : |j| = depth h)
-  : (h,j) ∈ t.
-Proof.
-  assert (depth h <= | i |) as Hdepi.
-  {
-    eapply tag_depth' in Hpath. rewrite Hpath.
-    eapply deq_loop_depth.
-    eapply loop_contains_deq_loop;eauto.
-  }
-  eapply loop_tag_dom_eq in Hpath as Hel2.
-  3: reflexivity.
-  2: eauto.
-  2: rewrite take_r_length_le;eauto.
-  eapply path_to_elem in Hel2;eauto.
-  destructH.
-  eapply prefix_incl;eauto.
-  eapply loop_tag_dom_same;eauto.
-  eapply loop_contains_loop_head;eauto.
-Qed.
 
 Section disj.
 
   Infix "-->" := edge__P.
-
 
   Context `(D : DiamondPaths).
   Hypothesis (Hjle : j1 ⊴ j2).
@@ -189,32 +12,7 @@ Section disj.
     : deq_loop s q1.
   Proof.
     clear Hjle.
-    intros h Hh.
-    eapply loop_contains_innermost in Hh as Hinner. destructH.
-    eapply eq_loop_innermost in Hinner as Hinner'. 2: eapply Dloop.
-    eapply innermost_loop_deq_loop;eauto. 2:eapply Dloop in Hh;auto.
-    destruct r1, r2; inv_Dpaths D.
-    1-3: lazymatch goal with
-         | H : innermost_loop ?h' s |- _ => destruct H;eauto
-         end.
-    decide (loop_contains h' s);[assumption|exfalso].
-    copy Hinner Hinner''.
-    eapply Dpath_sq1 in D as Hsq1.
-    eapply Dpath_sq2 in D as Hsq2.
-    eapply ex_entry_innermost in Hinner;eauto.
-    2: eapply Dlen.
-    eapply ex_entry_innermost in Hinner';eauto.
-    2: eapply Dlen.
-    eapply tl_eq in D as Htl.
-    rewrite Htl in Hinner.
-    eapply In_rcons in Hinner.
-    eapply In_rcons in Hinner'.
-    destruct Hinner, Hinner'.
-    1-3: lazymatch goal with
-         | H: (?h', _ ) = (s,k) |- _ => inv H
-         end;
-      eapply n;destruct Hinner'';eauto using loop_contains_self.
-    eapply Ddisj;eauto.
+    eapply diamond_split in D. eapply spath_s_deq_q;eauto.
   Qed.
 
   Lemma no_head_inst (h : Lab) (l : Tag)
@@ -222,145 +20,12 @@ Section disj.
         (Hel : (h,l) ∈ r1)
     : False.
   Proof.
-    specialize (tcfg_reachability Dlen) as Hreach.
-    specialize Dpath1 as Dpath1'.
-    destructH.
-    specialize Dpath1 as Hpath1.
-    eapply path_app in Hpath1. 2: eapply Hreach. 2: eapply Dsk1.
-    cbn in Hpath1.
-    destruct r1;[contradiction|].
-    inv_Dpaths D.
-    inv_path Hpath1.
-    assert (|j1| = depth h) as Hheq.
-    { eapply innermost_eq_loop in Hcont;rewrite Hcont. eapply j_len1;eauto. }
-    assert (|j2| = depth h) as Hheq2.
-    { eapply jj_len in D. rewrite <-D. assumption. }
-    eapply loop_tag_dom_eq in H as Hin;eauto. 2: destruct Hcont;eauto.
-    2: rewrite take_r_geq;rewrite Hheq;eauto.
-    rewrite app_comm_cons in Hin.
-    eapply in_app_or in Hin.
-    rewrite take_r_geq in Hin.
-    2: { eapply innermost_eq_loop in Hcont. rewrite Hcont. erewrite <-j_len1;eauto. }
-    assert ((h,j1) ∉ t) as Hnin.
-    - intro N.
-      eapply path_from_elem in N;eauto. destructH.
-      inv_path Dpath1'.
-      eapply path_from_elem in Hel as Helfrom;eauto. destructH.
-      eapply path_to_elem in Hel;eauto.
-      destructH.
-      eapply tag_depth_unroot in Hel0 as Hhdep;eauto with diamond.
-      copy Hel0 Hϕ1.
-      eapply path_app in Hel0. 3: eapply Dsk1. 2: eapply N0.
-      copy Hel0 Hel0'.
-      eapply tagle_monotone in Hel0;eauto.
-      2,3: reflexivity.
-      do 2 rewrite take_r_geq in Hel0. all: try rewrite Hheq;eauto.
-      2: rewrite <-Hhdep;eauto.
-      eapply tagle_monotone in Helfrom0;eauto.
-      2: reflexivity.
-      2: eapply loop_contains_deq_loop;destruct Hcont;eauto.
-      do 2 rewrite take_r_geq in Helfrom0;eauto. all: try rewrite Hheq;try rewrite Hhdep;eauto.
-      assert (j1 = l) as Heq.
-      + eapply partial_order_antisym;eauto.
-      + eapply tcfg_fresh in Hel0';eauto.
-        * subst l. eapply Taglt_irrefl;eauto.
-        * inv_path N0; inv_path Hϕ1;cbn;try rewrite app_length;cbn;lia.
-    - destruct Hin as [Hin|Hin]. 2: eapply Hnin;eauto.
-      enough (Hin2 : (h, j1) ∈ r2).
-      { eapply Ddisj;eauto. }
-      specialize Dpath2 as Hpath2.
-      eapply path_app in Hpath2. 2: eapply Hreach. 2: eapply Dsk2.
-      enough ((h,j1) ∈ (r2 ++ t)).
-      { eapply in_app_or in H1. destruct H1 as [H1|Hin2];[eauto|exfalso;eapply Hnin;eauto]. }
-      cbn in Hpath2.
-      inversion Hpath2.
-      { subst p2 i. subst a. symmetry in H5. eapply app_eq_nil in H5. destructH. subst t. inv Hreach. }
-      subst.
-      assert (b = (q2,j2)).
-      { destruct b as [q j]. destruct r2.
-        - setoid_rewrite <-Dqj2. cbn. cbn in H2. inv_path Hreach;inv H2;eauto.
-        - setoid_rewrite <-Dqj2. cbn. cbn in H2; inv_path H2;eauto.
-      }
-      subst b.
-      eapply loop_tag_dom;eauto.
-      + rewrite <-Dloop. destruct Hcont;eassumption.
-      + rewrite take_r_geq;[|rewrite <-Hheq2;eauto].
-        eauto with diamond.
-  Qed.
-
-  Lemma r1_incl_head_q' : forall x, x ∈ map fst r1 -> deq_loop x q1.
-    intros x Hel h Hh.
-    eapply loop_contains_innermost in Hh as Hinner1. destructH.
-    eapply eq_loop_innermost in Hinner1 as Hinner2. 2: eapply Dloop.
-    eapply innermost_loop_deq_loop;eauto. 2: rewrite <-Dloop;eauto.
-    decide (loop_contains h' x);[auto|exfalso].
-    eapply in_fst in Hel as Hfst.
-    destruct Hfst as [b Hfst].
-    eapply path_from_elem in Hfst. destructH. 2:eauto. 2: eapply Dpath_uq1;eauto.
-    2: intro N;rewrite N in Hel; cbn in Hel;contradiction.
-    eapply ex_entry_innermost in Hfst0 as Hentry;eauto.
-    2: { eapply tag_depth_unroot2;eauto with diamond. eapply j_len1;eauto. }
-    eapply postfix_incl in Hfst1. eapply Hfst1 in Hentry. exfalso.
-    eapply no_head_inst in Hentry as Hentry2;eauto.
-  Qed.
-
-  Lemma r2_incl_head_q' : forall x, x ∈ map fst r2 -> deq_loop x q1.
-  Proof.
-    intros x Hel h Hh.
-    eapply loop_contains_innermost in Hh as Hinner. destructH.
-    eapply eq_loop_innermost in Hinner as Hinner'; [|eapply Dloop];eauto.
-    eapply innermost_loop_deq_loop;eauto. 2:eapply Dloop in Hh;auto.
-    cbn. decide (loop_contains h' x);[auto|exfalso].
-    eapply in_fst in Hel. destructH.
-    destruct r2;[contradiction|].
-    inv_Dpaths D.
-    specialize Dpath2 as Dpath2'; inv_path Dpath2'.
-    eapply path_from_elem in Hel as Hϕ;eauto.
-    destructH.
-    assert (|b| = depth x) as Hbx.
-    { eapply path_to_elem in Hel;eauto. destructH. eapply tag_depth_unroot;eauto with diamond. }
-    eapply ex_entry_innermost in Hinner';eauto.
-    erewrite <-tl_eq in Hinner';eauto.
-    specialize (tcfg_reachability Dlen) as Hproot. destructH.
-    specialize Dpath1 as Hπ.
-    eapply path_app in Hπ. 3: eapply Dsk1. 2:eauto.
-    assert ((h', 0 :: tl j1) ∉ t) as Hnin.
-    - intro N.
-      eapply path_from_elem in N;eauto. destructH.
-      eapply postfix_incl in Hinner';eauto.
-      eapply path_to_elem in Hinner';eauto. destructH.
-      eapply path_app in Hinner'0 as Hel0'. 3: eapply Dsk2. 2:eapply N0.
-      eapply tcfg_fresh in Hel0'.
-      + eapply Taglt_irrefl;eauto.
-      + eapply innermost_eq_loop in Hinner. rewrite Hinner. setoid_rewrite <-j_len1. 2:eauto.
-        destruct j1;cbn;eauto.
-        exfalso. eapply loop_contains_depth_lt in Hh. setoid_rewrite <-j_len1 in Hh;eauto.
-        cbn in Hh. lia.
-      + destruct ϕ1,ϕ0;try rewrite app_length;cbn;try lia;inv Hinner'0;inv N0.
-    - specialize Dqj1 as Hqj1.
-      cbn in Hπ.
-      destruct r1;cbn in Hqj1.
-      + inv Hqj1. eapply ex_entry_innermost in Hproot;cbn;eauto.
-        * rewrite depth_root. eauto.
-        * eapply root_no_loop.
-      + subst p. inv_path Hπ.
-        eapply ex_entry_innermost in H1;cbn;eauto.
-        * rewrite app_comm_cons in H1. eapply in_app_or in H1. destruct H1;[|contradiction].
-          eapply Ddisj;eauto. eapply postfix_incl;eauto.
-        * rewrite depth_root. eauto.
-        * eapply root_no_loop.
+    eapply diamond_split in D. eapply spath_no_head_inst;eauto.
   Qed.
 
   Lemma no_back : forall x : Lab, x ∈ (map fst r1) -> ~ loop_contains x q1.
   Proof. (* Hjle needed *)
-    intros h' Hel Hnin.
-    eapply in_fst in Hel.
-    destructH.
-    decide (innermost_loop h' q1).
-    - eapply no_head_inst in Hel as Hel';eauto.
-    - simpl_dec' n.
-      destruct n;[contradiction|]. eapply H.
-      eapply r1_incl_head_q'. eapply in_map with (f:=fst) in Hel. cbn in Hel. assumption.
+    eapply diamond_split in D. eapply spath_no_back;eauto.
   Qed.
 
 End disj.
@@ -427,6 +92,20 @@ Proof.
     + exploit IHl. destructH. eexists. right. eassumption.
 Qed.
 
+Lemma r1_incl_head_q `(D : DiamondPaths)
+  : forall x, x ∈ map fst r1 -> deq_loop x q1.
+Proof.
+  eapply diamond_split in D.
+  eapply spath_r1_incl_head_q. eassumption.
+Qed.
+
+Lemma r2_incl_head_q `(D : DiamondPaths)
+  : forall x, x ∈ map fst r2 -> deq_loop x q1.
+Proof.
+  eapply diamond_split in D.
+  eapply spath_r2_incl_head_q. eassumption.
+Qed.
+
 Lemma tag_eq1 `(D : DiamondPaths)
       (Hjle : j1 ⊴ j2)
     : forall j, j ∈ map snd r1 -> take_r (depth q1) j = j1.
@@ -442,10 +121,10 @@ Lemma tag_eq1 `(D : DiamondPaths)
       + erewrite <-take_r_geq.
         * rewrite Hpath1'. eapply Hϕ0.
         * erewrite j_len1;eauto.
-      + intros. eapply r1_incl_head_q';eauto.
+      + intros. eapply r1_incl_head_q;eauto.
       + intros. eapply no_back;eauto.
     - eauto with diamond.
-    - intros. eapply r1_incl_head_q';eauto. eapply prefix_incl;eauto.
+    - intros. eapply r1_incl_head_q;eauto. eapply prefix_incl;eauto.
       eapply prefix_map_fst;eauto.
     - intros. eapply no_back;eauto. eapply prefix_incl;eauto. eapply prefix_map_fst;eauto.
   Qed.
@@ -491,7 +170,7 @@ Lemma tag_eq1 `(D : DiamondPaths)
             - exfalso. eapply n. cbn in *. eapply u_len1 in D as Hlen. rewrite Htag in Hlen.
               cbn in Hlen.
               eapply deq_loop_head_loop_contains.
-              + eapply deq_loop_depth_eq. eapply r1_incl_head_q';eauto. 2:lia.
+              + eapply deq_loop_depth_eq. eapply r1_incl_head_q;eauto. 2:lia.
                 destruct D. inv_path Dpath1. eapply path_contains_back in H0.
                 eapply in_map with (f:=fst) in H0. cbn in *. eauto.
               + eexists;eauto.
@@ -507,7 +186,7 @@ Lemma tag_eq1 `(D : DiamondPaths)
           erewrite take_r_cons_drop.
           -- subst. reflexivity.
           -- eapply u_len1 in D as Hlen. subst k. rewrite Hlen. eapply deq_loop_depth.
-             eapply r1_incl_head_q';eauto.
+             eapply r1_incl_head_q;eauto.
              destruct D. inv_path Dpath1. eapply path_contains_back in H.
              eapply in_map with (f:=fst) in H. cbn in *. eauto.
   Qed.
@@ -543,7 +222,7 @@ Lemma tag_eq1 `(D : DiamondPaths)
           eapply in_map with (f:=fst) in H. unfold fst in H at 1. eauto.
       - exfalso. destruct Hedge. eapply exit_not_deq in H;eauto.
         eapply eq_loop_exiting in H. rewrite H. transitivity q1;eauto.
-        eapply r1_incl_head_q';eauto.
+        eapply r1_incl_head_q;eauto.
         destruct D. inv_path Dpath1. eapply path_contains_back in H0.
         eapply in_map with (f:=fst) in H0. unfold fst in H0 at 1. eauto.
     Qed.
@@ -559,7 +238,7 @@ Lemma tag_eq1 `(D : DiamondPaths)
       - right. right. eapply loop_contains_ledge in Hedge. eapply Hdeq;eauto.
       - exfalso. destruct Hedge. eapply exit_not_deq in H;eauto.
         eapply eq_loop_exiting in H. rewrite H. transitivity q1;eauto.
-        eapply r2_incl_head_q';eauto.
+        eapply r2_incl_head_q;eauto.
         destruct D. inv_path Dpath2. eapply path_contains_back in H0.
         eapply in_map with (f:=fst) in H0. unfold fst in H0 at 1. eauto.
     Qed.
@@ -575,26 +254,6 @@ Proof.
   eapply no_back.
   - eapply DiamondPaths_sym;eauto.
   - subst. reflexivity.
-Qed.
-
-Lemma r1_incl_head_q `(D : DiamondPaths)
-  : forall x, x ∈ map fst r1 -> deq_loop x q1.
-Proof.
-  specialize (jj_len D) as Hlen.
-  eapply tagle_or in Hlen.
-  destruct Hlen.
-  - eapply r1_incl_head_q';eauto.
-  - setoid_rewrite Dloop.
-    eapply r2_incl_head_q';eauto.
-    eapply DiamondPaths_sym;eauto.
-Qed.
-
-Lemma r2_incl_head_q `(D : DiamondPaths)
-  : forall x, x ∈ map fst r2 -> deq_loop x q1.
-Proof.
-  setoid_rewrite Dloop.
-  eapply r1_incl_head_q.
-  eapply DiamondPaths_sym;eauto.
 Qed.
 
 Lemma u1_deq_q `(D : DiamondPaths)
