uniana/disj/SpathIncl.v
@@ -1,0 +1,421 @@
+Require Export DiamondPaths.
+Require Import Lia.
+
+Definition sub_tag i j := |i| = |j| /\ hd 0 i <= hd 0 j /\ tl i = tl j.
+
+Lemma Tagle_len: forall [i j : Tag], i ⊴ j -> | i | = | j |.
+Proof.
+  intros. destruct H.
+  - eapply Taglt_len;eauto.
+  - subst. reflexivity.
+Qed.
+
+Lemma spath_jj_subtag `(SplitPaths)
+      (Hjle : j1 ⊴ j2)
+  : sub_tag j1 j2.
+Proof.
+  split;[|split].
+  - eapply Tagle_len;eauto.
+  - destruct Hjle;[|subst;eauto].
+    destruct H0;cbn;try lia.
+    exfalso.
+    specialize Stl as Htl. cbn in Htl. subst. eapply Taglt_irrefl;eauto.
+  - eapply Stl.
+Qed.
+
+Lemma jj_subtag `(DiamondPaths)
+      (Hjle : j1 ⊴ j2)
+  : sub_tag j1 j2.
+Proof.
+  eapply diamond_split in H. eapply spath_jj_subtag;eauto.
+Qed.
+
+Hint Resolve jj_subtag : diamond.
+
+Lemma loop_tag_dom_eq `(C : redCFG) (h p : Lab) (i j : Tag) t
+      (Hloop : loop_contains h p)
+      (Hpath : TPath (root,start_tag) (p,i) t)
+      (Htagle : j = take_r (depth h) i)
+      (Hdep : |j| = depth h)
+  : (h,j) ∈ t.
+Proof.
+  subst j.
+  clear Hdep.
+  revert h p i Hloop Hpath.
+  induction t;intros.
+  + inv Hpath.
+  + unfold TPath in Hpath. path_simpl' Hpath. destruct t.
+    {
+      eapply path_single in Hpath. destruct Hpath.
+      inversion H. subst p i. eapply root_no_loop in Hloop. contradiction.
+    }
+    inv_path Hpath. destruct c as [q j].
+    specialize (IHt) with (p:=q) (i:=j).
+    eapply tcfg_edge_destruct' in H0.
+    destruct H0 as [H0|[H0|[H0|H0]]].
+    all: destruct H0 as [Htag Hedge].
+    * subst. right.
+      eapply IHt. all:cycle 1.
+      -- eapply H.
+      -- eapply basic_edge_eq_loop in Hedge. rewrite Hedge. assumption.
+    * eapply deq_loop_entry_or in Hedge;eauto.
+      destruct Hedge.
+      -- subst. right.
+         rewrite take_r_cons_drop.
+         2: {
+           eapply loop_contains_deq_loop in H0.
+           eapply tag_depth' in H. rewrite H.
+           eapply deq_loop_depth;eauto.
+         }
+         eapply IHt;eauto.
+      -- subst p. left. rewrite take_r_geq;eauto.
+         eapply tag_depth' in Hpath. lia.
+    * destruct j.
+      {
+        eapply tag_depth' in H. cbn in H. eapply loop_contains_depth_lt in Hloop.
+        eapply back_edge_eq_loop in Hedge. rewrite Hedge in H. lia.
+      }
+      cbn in Htag. subst i.
+      decide (h = p).
+      -- subst p. left. rewrite take_r_geq;eauto.
+         eapply tag_depth' in Hpath. lia.
+      -- right. rewrite take_r_cons_replace with (b:=n).
+         2: {
+           copy Hedge Hedge'.
+           eapply back_edge_eq_loop in Hedge.
+           copy Hloop Hloop'.
+           eapply loop_contains_deq_loop in Hloop.
+           eapply eq_loop1 in Hloop;eauto. 2: symmetry;eauto.
+           eapply tag_depth' in H.
+           enough (depth h < S (| j |)).
+           { cbn in H. rewrite H in H0. lia. }
+           eapply deq_loop_depth in Hloop.
+           eapply le_lt_or_eq in Hloop.
+           destruct Hloop.
+           ++ cbn in H. lia.
+           ++ exfalso. rewrite Hedge in H0.
+              eapply loop_contains_deq_loop in Hloop' as Hdeq.
+              eapply deq_loop_depth_eq in H0;eauto.
+              eapply n0. eapply head_unique;eauto.
+              ** eapply loop_contains_ledge;eauto.
+              ** split;eauto.
+         }
+         eapply IHt;eauto.
+         eapply back_edge_eq_loop in Hedge. rewrite Hedge. eauto.
+    * subst.
+      destruct j.
+      {
+        eapply tag_depth' in H. cbn in H. eapply loop_contains_depth_lt in Hloop.
+        destruct Hedge. eapply deq_loop_exited in H0. eapply deq_loop_depth in H0. lia.
+      }
+      right. rewrite <-take_r_cons_drop with (a:=n).
+      all: cbn.
+      2: {
+        eapply tag_depth' in H. cbn in H.
+        enough (depth h < S (|j|)) by lia.
+        rewrite H.
+        eapply depth_exit in Hedge.
+        eapply loop_contains_deq_loop in Hloop. eapply deq_loop_depth in Hloop.
+        lia.
+      }
+      eapply IHt;eauto.
+      destruct Hedge. eapply deq_loop_exited in H0. eapply H0. eauto.
+Qed.
+
+Lemma loop_tag_dom_same `(C : redCFG) (h : Lab) (i j : Tag) t
+      (Hloop : loop_head h)
+      (Hpath : TPath (root,start_tag) (h,i) t)
+      (Htagle : sub_tag j i)
+  : (h,j) ∈ t.
+Proof.
+  destruct Htagle as [Hlen [Hhd Htl]].
+  destruct i,j;cbn in *;[|congruence|congruence|].
+  { eapply tag_depth' in Hpath. cbn in Hpath. eapply depth_loop_head in Hloop. lia. }
+  subst j. clear Hlen.
+  revert t Hpath.
+  induction Hhd;intros.
+  - eapply path_contains_front;eauto.
+  - destruct t;[inv Hpath|].
+    unfold TPath in Hpath. path_simpl' Hpath.
+    inversion Hpath. subst.
+    destruct b as [q j].
+    eapply tcfg_edge_destruct' in H3.
+      destruct H3 as [H3|[H3|[H3|H3]]].
+      all: destruct H3 as [Htag Hedge].
+      * eapply basic_edge_no_loop2 in Hedge. contradiction.
+      * inv Htag.
+      * destruct j;cbn in Htag;[congruence|].
+        inv Htag.
+        right.
+        eapply loop_tag_dom_eq in H0 as Hel2;cycle 1.
+        -- eapply loop_contains_ledge;eassumption.
+        -- rewrite take_r_geq;eauto. eapply tag_depth' in H0. rewrite H0.
+           eapply back_edge_eq_loop in Hedge. rewrite Hedge. eauto.
+        -- eapply back_edge_eq_loop in Hedge. rewrite <-Hedge. eapply tag_depth' in H0. eauto.
+        -- eapply path_to_elem in Hel2;eauto. destructH.
+           eapply prefix_incl;[eauto|].
+           eapply IHHhd;eassumption.
+      * destruct j;cbn in Htag;[congruence|]. subst j. destruct Hedge.
+        eapply no_exit_head in H. contradiction.
+Qed.
+
+(* could be generalized with sub_tag _ _  -> sub_tag _ _ \/ Prefix _ _ *)
+Lemma loop_tag_dom `(C : redCFG) (h p : Lab) (i j : Tag) t
+      (Hloop : loop_contains h p)
+      (Hpath : TPath (root,start_tag) (p,i) t)
+      (Hstag : sub_tag j (take_r (depth h) i))
+      (Hdep : |j| = depth h)
+  : (h,j) ∈ t.
+Proof.
+  assert (depth h <= | i |) as Hdepi.
+  {
+    eapply tag_depth' in Hpath. rewrite Hpath.
+    eapply deq_loop_depth.
+    eapply loop_contains_deq_loop;eauto.
+  }
+  eapply loop_tag_dom_eq in Hpath as Hel2.
+  3: reflexivity.
+  2: eauto.
+  2: rewrite take_r_length_le;eauto.
+  eapply path_to_elem in Hel2;eauto.
+  destructH.
+  eapply prefix_incl;eauto.
+  eapply loop_tag_dom_same;eauto.
+  eapply loop_contains_loop_head;eauto.
+Qed.
+
+Hint Resolve Spath1 Spath2 Sdisj Sloop Stl Slen : spath.
+
+Section spath.
+  Context `(S : SplitPaths).
+
+  Lemma spath_j_len1
+    : | j1 | = depth q1.
+  Proof.
+    eapply tag_depth_unroot;eauto with spath. eapply Spath1.
+  Qed.
+
+  Lemma spath_j_len2
+    : | j2 | = depth q2.
+  Proof.
+    eapply tag_depth_unroot;eauto with spath. eapply Spath2.
+  Qed.
+
+  Lemma spath_jj_len
+    : |j1| = |j2|.
+  Proof.
+    erewrite spath_j_len1.
+    erewrite spath_j_len2.
+    rewrite Sloop. reflexivity.
+  Qed.
+
+  Lemma spath_s_deq_q
+    : deq_loop s q1.
+  Proof.
+    intros h Hh.
+    eapply loop_contains_innermost in Hh as Hinner. destructH.
+    eapply eq_loop_innermost in Hinner as Hinner'. 2: eapply Sloop.
+    eapply innermost_loop_deq_loop;eauto. 2:eapply Sloop in Hh;auto.
+    decide (loop_contains h' s);[assumption|exfalso].
+    copy Hinner Hinner''.
+    eapply ex_entry_innermost in Hinner;eauto with spath. 2: eapply Spath1.
+    eapply ex_entry_innermost in Hinner';eauto with spath. 2: eapply Spath2.
+    rewrite Stl in Hinner.
+    eapply In_rcons in Hinner. eapply In_rcons in Hinner'.
+    destruct Hinner, Hinner'.
+    1-3: lazymatch goal with
+         | H: (?h', _ ) = (s,k) |- _ => inv H
+         end;
+      eapply n;destruct Hinner'';eauto using loop_contains_self.
+    eapply Sdisj;eauto.
+  Qed.
+
+  Lemma spath_no_head_inst (h : Lab) (l : Tag)
+        (Hjle : j1 ⊴ j2)
+        (Hcont : innermost_loop h q1)
+        (Hel : (h,l) ∈ r1)
+    : False.
+  Proof.
+    specialize (tcfg_reachability Slen) as Hreach.
+    specialize Spath1 as Dpath1'.
+    destructH.
+    specialize Spath1 as Hpath1.
+    eapply path_app' in Hpath1. 2: eapply Hreach.
+    cbn in Hpath1.
+    assert (|j1| = depth h) as Hheq.
+    { eapply innermost_eq_loop in Hcont;rewrite Hcont. eapply spath_j_len1;eauto. }
+    assert (|j2| = depth h) as Hheq2.
+    { rewrite <-spath_jj_len. assumption. }
+    eapply loop_tag_dom_eq in Hpath1 as Hin;eauto. 2: destruct Hcont;eauto.
+    2: rewrite take_r_geq;rewrite Hheq;eauto.
+    rewrite <-app_assoc in Hin.
+    eapply in_app_or in Hin.
+    rewrite take_r_geq in Hin.
+    2: { eapply innermost_eq_loop in Hcont. rewrite Hcont. erewrite <-spath_j_len1;eauto. }
+    rewrite <-app_assoc in Hpath1.
+    assert ([(s,k)] ++ tl t = t) as Hsktlt.
+    { destruct t;[inv Hreach|]. cbn. unfold TPath in Hreach. path_simpl' Hreach. reflexivity. }
+    replace ([(s,k)] ++ tl t) with t in Hpath1, Hin by eauto.
+    assert ((h,j1) ∉ t) as Hnin.
+    - intro N.
+      eapply path_from_elem in N;eauto. destructH.
+      specialize Spath1 as Spath1'.
+      destruct r1;[contradiction|]. cbn in Spath1'. unfold TPath in Spath1'. path_simpl' Spath1'.
+      eapply path_rcons_inv' in Spath1' as Sedge.
+      destructH.
+      eapply path_from_elem in Hel as Helfrom;eauto.
+      destructH.
+      copy Hel Hel'.
+      eapply path_to_elem in Hel;eauto.
+      destructH.
+      assert (|l| = depth h) as Hhdep.
+      { eapply path_to_elem in Dpath1'. 2: rewrite In_rcons;right;eauto. destructH.
+        eapply tag_depth_unroot in Dpath1'0;eauto with spath. }
+      copy Hel0 Hϕ1.
+      eapply path_app in Hel0. 3:eauto. 2: eapply N0.
+      copy Hel0 Hel0'.
+      eapply tagle_monotone in Hel0;eauto.
+      2,3: reflexivity.
+      do 2 rewrite take_r_geq in Hel0. all: try rewrite Hheq;eauto.
+      2: rewrite <-Hhdep;eauto.
+      eapply tagle_monotone in Helfrom0;eauto.
+      2: reflexivity.
+      2: eapply loop_contains_deq_loop;destruct Hcont;eauto.
+      do 2 rewrite take_r_geq in Helfrom0;eauto. all: try rewrite Hheq;try rewrite Hhdep;eauto.
+      assert (j1 = l) as Heq.
+      + eapply partial_order_antisym;eauto.
+      + eapply tcfg_fresh in Hel0';eauto.
+        * subst l. eapply Taglt_irrefl;eauto.
+        * inv_path N0; inv_path Hϕ1;cbn;try rewrite app_length;cbn;lia.
+    - destruct Hin as [Hin|Hin]. 2: eapply Hnin;eauto.
+      enough (Hin2 : (h, j1) ∈ r2).
+      { eapply Sdisj;eauto. }
+      specialize Spath2 as Hpath2.
+      eapply path_app' in Hpath2. 2: eapply Hreach.
+      rewrite <-app_assoc in Hpath2.
+      rewrite Hsktlt in Hpath2.
+      enough ((h,j1) ∈ (r2 ++ t)).
+      { eapply in_app_or in H. destruct H as [H1|Hin2];[eauto|exfalso;eapply Hnin;eauto]. }
+      cbn in Hpath2.
+      eapply loop_tag_dom;eauto.
+      + rewrite <-Sloop. destruct Hcont;eassumption.
+      + rewrite take_r_geq;[|rewrite <-Hheq2;eauto].
+        eapply spath_jj_subtag;eauto.
+  Qed.
+
+End spath.
+
+Lemma spath_r1_incl_head_q' `(S : SplitPaths)
+      (Hjle : j1 ⊴ j2)
+  : forall x, x ∈ map fst r1 -> deq_loop x q1.
+  intros x Hel h Hh.
+  eapply loop_contains_innermost in Hh as Hinner1. destructH.
+  eapply eq_loop_innermost in Hinner1 as Hinner2. 2: eapply Sloop.
+  eapply innermost_loop_deq_loop;eauto. 2: rewrite <-Sloop;eauto.
+  decide (loop_contains h' x);[auto|exfalso].
+  eapply in_fst in Hel as Hfst.
+  destruct Hfst as [b Hfst].
+  destruct r1;[contradiction|].
+  specialize Spath1 as Spath1'. cbn in Spath1'. unfold TPath in Spath1'. path_simpl' Spath1'.
+  eapply path_rcons_inv in Spath1'. destructH.
+  eapply path_from_elem in Hfst. destructH. 2:eauto. 2: eapply Spath1'.
+  eapply ex_entry_innermost in Hfst0 as Hentry;eauto.
+  2: { eapply tag_depth_unroot2;eauto with spath. eapply spath_j_len1;eauto. }
+  eapply postfix_incl in Hfst1. eapply Hfst1 in Hentry. exfalso.
+  eapply spath_no_head_inst in Hentry as Hentry2;eauto.
+Qed.
+
+Lemma spath_r2_incl_head_q' `(S : SplitPaths)
+      (Hjle : j1 ⊴ j2)
+  : forall x, x ∈ map fst r2 -> deq_loop x q1.
+Proof.
+  intros x Hel h Hh.
+  eapply loop_contains_innermost in Hh as Hinner. destructH.
+  eapply eq_loop_innermost in Hinner as Hinner'; [|eapply Sloop];eauto.
+  eapply innermost_loop_deq_loop;eauto. 2:eapply Sloop in Hh;auto.
+  cbn. decide (loop_contains h' x);[auto|exfalso].
+  eapply in_fst in Hel. destructH.
+  destruct r2;[contradiction|].
+  specialize Spath2 as Dpath2'. cbn in Dpath2'. unfold TPath in Dpath2'.
+  path_simpl' Dpath2'. eapply path_rcons_inv' in Dpath2'. destructH.
+  eapply path_from_elem in Hel as Hϕ;eauto.
+  destructH.
+  assert (|b| = depth x) as Hbx.
+  { eapply tag_depth_unroot2;eauto with spath. eapply spath_j_len2;eauto. }
+  eapply ex_entry_innermost in Hinner';eauto.
+  erewrite <-Stl in Hinner';eauto.
+  specialize (tcfg_reachability Slen) as Hproot. destructH.
+  specialize Spath1 as Hπ.
+  eapply path_app' in Hπ. 2: eapply Hproot.
+  assert ([(s,k)] ++ tl t = t) as Hsktlt.
+  { destruct t;[inv Hproot|]. cbn. unfold TPath in Hproot. path_simpl' Hproot. reflexivity. }
+  rewrite <-app_assoc in Hπ.
+  rewrite Hsktlt in Hπ.
+  assert ((h', 0 :: tl j1) ∉ t) as Hnin.
+  - intro N.
+    eapply path_from_elem in N;eauto. destructH.
+    eapply postfix_incl in Hinner';eauto.
+    eapply path_to_elem in Hinner';eauto. destructH.
+    eapply path_app in Hinner'0 as Hel0'. 3: eauto. 2:eapply N0.
+    eapply tcfg_fresh in Hel0'.
+    + eapply Taglt_irrefl;eauto.
+    + eapply innermost_eq_loop in Hinner. rewrite Hinner. setoid_rewrite <-spath_j_len1. 2:eauto.
+      destruct j1;cbn;eauto.
+      exfalso. eapply loop_contains_depth_lt in Hh. setoid_rewrite <-spath_j_len1 in Hh;eauto.
+      cbn in Hh. lia.
+    + destruct ϕ1,ϕ0;try rewrite app_length;cbn;try lia;inv Hinner'0;inv N0.
+  - specialize Spath1 as Spath1'. destruct r1.
+    + cbn in Spath1'. eapply path_single in Spath1'. destructH. inv Spath1'0. inv Spath1'1.
+      eapply ex_entry_innermost in Hproot;cbn;eauto.
+      * rewrite depth_root. eauto.
+      * eapply root_no_loop.
+    + cbn in Spath1'. unfold TPath in Spath1'. path_simpl' Spath1'. inv_path Spath1'. congruence'.
+      eapply ex_entry_innermost in Hπ;cbn;eauto.
+      * eapply in_app_or in Hπ. destruct Hπ;[|contradiction].
+        eapply Sdisj;eauto. eapply postfix_incl;eauto.
+      * rewrite depth_root. eauto.
+      * eapply root_no_loop.
+Qed.
+
+Lemma spath_no_back `(S : SplitPaths)
+      (Hjle : j1 ⊴ j2)
+  : forall x : Lab, x ∈ (map fst r1) -> ~ loop_contains x q1.
+Proof. (* Hjle needed *)
+  intros h' Hel Hnin.
+  eapply in_fst in Hel.
+  destructH.
+  decide (innermost_loop h' q1).
+  - eapply spath_no_head_inst in Hel as Hel';eauto.
+  - simpl_dec' n.
+    destruct n;[contradiction|]. eapply H.
+    eapply spath_r1_incl_head_q';eauto. eapply in_map with (f:=fst) in Hel. cbn in Hel. assumption.
+Qed.
+
+Lemma SplitPaths_sym `(S : SplitPaths)
+  : SplitPaths s q2 q1 k j2 j1 r2 r1.
+Proof.
+  econstructor.
+  3: eapply Disjoint_sym.
+  4,5: symmetry.
+  all: eauto with spath.
+Qed.
+
+Lemma spath_r1_incl_head_q `(S : SplitPaths)
+  : forall x, x ∈ map fst r1 -> deq_loop x q1.
+Proof.
+  specialize (spath_jj_len S) as Hlen.
+  eapply tagle_or in Hlen.
+  destruct Hlen.
+  - eapply spath_r1_incl_head_q';eauto.
+  - setoid_rewrite Sloop.
+    eapply spath_r2_incl_head_q';eauto.
+    eapply SplitPaths_sym;eauto.
+Qed.
+
+Lemma spath_r2_incl_head_q `(S : SplitPaths)
+  : forall x, x ∈ map fst r2 -> deq_loop x q1.
+Proof.
+  setoid_rewrite Sloop.
+  eapply spath_r1_incl_head_q.
+  eapply SplitPaths_sym;eauto.
+Qed.
